Added exact lemma for parameteriezed global hybrids.
Added global hybrid lemma for hybrids parameterized by
oracles that gives an equality, not just an upper bound.
Updated the DDH global hybrid example to use it. Idea based on the
Nominal-SSProve paper "Mechanizing Nested Hybrid
Arguments", https://eprint.iacr.org/2025/1122.

examples/global-hybrid/GlobalHybridExamp2.ec
@@ -1,49 +1,45 @@
 (* GlobalHybridExamp2.ec *)
 
-(* We use theories/crypto/GlobalHybrid.ec for an example where the
-   cost of each hybrid step is an instance of the Decisional
-   Diffie-Hellman (DDH) assumption. *)
+(* We use theories/crypto/GlobalHybrid.ec for an example involving the
+   Decisional Diffie-Hellman (DDH) assumption, expressing security
+   as an equality. *)
 
-require import AllCore Real Distr DBool StdOrder StdBigop GlobalHybrid.
+require import AllCore Real Distr DBool StdOrder StdBigop.
 require import FMap PROM.
 import RealOrder Bigreal BRA.
+require GlobalHybrid.
+
+theory DDH.
+
+type input.  (* additional input *)
 
 (* group of keys *)
 
 type key.
 
 op (^^) : key -> key -> key.  (* binary operation *)
-
-op kid : key.  (* identity *)
-
-op kinv : key -> key.  (* inverse *)
+op kid  : key.                (* identity *)
+op kinv : key -> key.         (* inverse *)
 
 axiom kmulA (x y z : key) : x ^^ y ^^ z = x ^^ (y ^^ z).
-
-axiom kid_l (x : key) : kid ^^ x = x.
-
-axiom kid_r (x : key) : x ^^ kid = x.
-
-axiom kinv_l (x : key) : kinv x ^^ x = kid.
-
-axiom kinv_r (x : key) : x ^^ kinv x = kid.
+axiom kid_l (x : key)     : kid ^^ x = x.
+axiom kid_r (x : key)     : x ^^ kid = x.
+axiom kinv_l (x : key)    : kinv x ^^ x = kid.
+axiom kinv_r (x : key)    : x ^^ kinv x = kid.
 
 (* commutative semigroup of exponents *)
 
 type exp.
 
-op e : exp.  (* some exponent *)
-
+op e     : exp.  (* some exponent *)
 op ( * ) : exp -> exp -> exp.  (* multiplication *)
 
-axiom mulC (q r : exp) : q * r = r * q.
-
+axiom mulC (q r : exp)   : q * r = r * q.
 axiom mulA (q r s : exp) : q * r * s = q * (r * s).
 
 op [full uniform lossless] dexp : exp distr.
 
-op g : key.  (* generator *)
-
+op g   : key.  (* generator *)
 op (^) : key -> exp -> key.  (* exponentiation *)
 
 axiom double_exp_gen (q1 q2 : exp) : (g ^ q1) ^ q2 = g ^ (q1 * q2).
@@ -51,30 +47,88 @@ axiom double_exp_gen (q1 q2 : exp) : (g ^ q1) ^ q2 = g ^ (q1 * q2).
 (* DDH Adversary *)
 
 module type DDH_ADV = {
-  proc main(k1 k2 k3 : key) : bool
+  proc main(i : input, k1 k2 k3 : key) : bool
 }.
 
 (* the real DDH game *)
 
 module DDH1 (Adv : DDH_ADV) = {
-  proc main() : bool = {
+  proc main(i : input) : bool = {
     var b : bool; var q1, q2 : exp;
     q1 <$ dexp; q2 <$ dexp;
-    b <@ Adv.main(g ^ q1, g ^ q2, g ^ (q1 * q2));
+    b <@ Adv.main(i, g ^ q1, g ^ q2, g ^ (q1 * q2));
     return b;
   }
 }.
-  
+
 (* the ideal DDH game *)
 
 module DDH2 (Adv : DDH_ADV) = {
-  proc main() : bool = {
+  proc main(i : input) : bool = {
     var b : bool; var q1, q2, q3 : exp;
     q1 <$ dexp; q2 <$ dexp; q3 <$ dexp;
-    b <@ Adv.main(g ^ q1, g ^ q2 , g ^ q3);
+    b <@ Adv.main(i, g ^ q1, g ^ q2 , g ^ q3);
     return b;
   }
 }.
+
+end DDH.
+
+(* group of keys *)
+
+type key.
+
+op (^^) : key -> key -> key.  (* binary operation *)
+op kid  : key.                (* identity *)
+op kinv : key -> key.         (* inverse *)
+
+axiom kmulA (x y z : key) : x ^^ y ^^ z = x ^^ (y ^^ z).
+axiom kid_l (x : key)     : kid ^^ x = x.
+axiom kid_r (x : key)     : x ^^ kid = x.
+axiom kinv_l (x : key)    : kinv x ^^ x = kid.
+axiom kinv_r (x : key)    : x ^^ kinv x = kid.
+
+(* commutative semigroup of exponents *)
+
+type exp.
+
+op e     : exp.  (* some exponent *)
+op ( * ) : exp -> exp -> exp.  (* multiplication *)
+
+axiom mulC (q r : exp)   : q * r = r * q.
+axiom mulA (q r s : exp) : q * r * s = q * (r * s).
+
+op [full uniform lossless] dexp : exp distr.
+
+op g   : key.  (* generator *)
+op (^) : key -> exp -> key.  (* exponentiation *)
+
+axiom double_exp_gen (q1 q2 : exp) : (g ^ q1) ^ q2 = g ^ (q1 * q2).
+
+clone import DDH as DDH' with
+  type input <- int,  (* note *)
+  type key   <- key,
+  type exp   <- exp,
+  op (^^)    <- (^^),
+  op kid     <- kid,
+  op kinv    <- kinv,
+  op e       <- e,
+  op ( * )   <- ( * ),
+  op dexp    <- dexp,
+  op g       <- g,
+  op (^)     <- (^)
+proof *.
+realize kmulA. apply kmulA. qed.
+realize kid_l. apply kid_l. qed.
+realize kid_r. apply kid_r. qed.
+realize kinv_l. apply kinv_l. qed.
+realize kinv_r. apply kinv_r. qed.
+realize mulC. apply mulC. qed.
+realize mulA. apply mulA. qed.
+realize dexp_ll. apply dexp_ll. qed.
+realize dexp_uni. apply dexp_uni. qed.
+realize dexp_fu. apply dexp_fu. qed.
+realize double_exp_gen. apply double_exp_gen. qed.
 
 (* the real and ideal games let an adversary call an oracle
    m times before the returned results return a default value *)
@@ -92,20 +146,16 @@ module OrReal : OR = {
   var ctr : int
   var x, y : exp
 
-  proc init() : unit = {
-    ctr <- 0;
-  }
+  proc init() : unit = { ctr <- 1; }
 
   proc get() : key * key * key = {
     var r : key * key * key;
-    if (ctr < m) {
+    if (ctr <= m) {
       x <$ dexp; y <$ dexp;
       r <- (g ^ x, g ^ y, g ^ (x * y));
       ctr <- ctr + 1;
     }
-    else {
-      r <- witness;
-    }
+    else { r <- witness; }
     return r;
   }
 }.
@@ -115,21 +165,17 @@ module OrReal : OR = {
 module OrIdeal : OR = {
   var ctr : int
 
-  proc init() : unit = {
-    ctr <- 0;
-  }
+  proc init() : unit = { ctr <- 1; }
 
   proc get() : key * key * key = {
     var r : key * key * key;
     var x, y, z : exp;
-    if (ctr < m) {
+    if (ctr <= m) {
       x <$ dexp; y <$ dexp; z <$ dexp;
       r <- (g ^ x, g ^ y, g ^ z);
       ctr <- ctr + 1;
     }
-    else {
-      r <- witness;
-    }
+    else { r <- witness; }
     return r;
   }
 }.
@@ -165,7 +211,7 @@ module GIdeal(Adv : ADV) = {
 (* our reduction to DDH *)
 
 module Reduct(Adv : ADV) : DDH_ADV = {
-  var i : int  (* needs to be a global to support game hoping *)
+  var i : int
   var u, v, w : key
 
   module Or = {
@@ -176,75 +222,82 @@ module Reduct(Adv : ADV) : DDH_ADV = {
     proc get() : key * key * key = {
       var r : key * key * key;
       var x, y, z : exp;
-      if (ctr < m) {
-        if (ctr + 1 < i) {
+      if (ctr <= m) {
+        if (ctr < i) {
           x <$ dexp; y <$ dexp; z <$ dexp;
           r <- (g ^ x, g ^ y, g ^ z);
         }
-        elif (ctr + 1 = i) {
-          r <- (u, v, w);
-        }
+        elif (ctr = i) { r <- (u, v, w); }
         else {
           x <$ dexp; y <$ dexp;
           r <- (g ^ x, g ^ y, g ^ (x * y));
         }
         ctr <- ctr + 1;
       }
-      else {
-        r <- witness;
-      }
+      else { r <- witness; }
       return r;
     }
   }
 
-  proc main(u' : key, v' : key, w' : key) : bool = {
-    var b : bool;
-    Or.ctr <- 0;
-    u <- u'; v <- v'; w <- w';
+  proc main(i' : int, u' : key, v' : key, w' : key) : bool = {
+    var b : bool; var x : unit;
+    Or.ctr <- 1;
+    i <- i'; u <- u'; v <- v'; w <- w';
     b <@ Adv(Or).disting();
     return b;
   }
 }.
 
-(* the reduction composed with DDH1 *)
-
-module DDH1Reduct(Adv : ADV) = {
-  proc main(i : int) : bool = {
-    var b : bool;
-    Reduct.i <- i;  (* so value of Reduct.i in memory irrelevant *)
-    b <@ DDH1(Reduct(Adv)).main();
-    return b;
-  }
-}.
-    
-(* the reduction composed with DDH2 *)
-
-module DDH2Reduct(Adv : ADV) = {
-  proc main(i : int) : bool = {
-    var b : bool;
-    Reduct.i <- i;  (* so value of Reduct.i in memory irrelevant *)
-    b <@ DDH2(Reduct(Adv)).main();
-    return b;
-  }
-}.
-
-(* our goal is to prove:
+(* We will prove security with an exact upper bound:
 
 lemma GReal_GIdeal (Adv <: ADV{-OrReal, -OrIdeal, -Reduct}) &m :
   `|Pr[GReal(Adv).main() @ &m : res] -
-    Pr[GIdeal(Adv).main() @ &m : res]| <=
-  bigi predT
-  (fun i =>
-   `|Pr[DDH1Reduct(Adv).main(i) @ &m : res] -
-     Pr[DDH2Reduct(Adv).main(i) @ &m : res]|)
-  1 (m + 1).
+    Pr[GIdeal(Adv).main() @ &m : res]| =
+  m%r *
+  `|bigi predT
+    (fun (i : int) =>
+       Pr[DDH1(Reduct(Adv)).main(i) @ &m : res] / m%r)
+    1 (m + 1) -
+    bigi predT
+    (fun (i : int) =>
+       Pr[DDH2(Reduct(Adv)).main(i) @ &m : res] / m%r)
+    1 (m + 1)|.
 *)
 
 section.
 
+local clone GlobalHybrid as GH with
+  type input <- unit
+proof *.
+
+local clone GH.Param as GHP with
+  type or_input  <- unit,
+  type or_output <- key * key * key
+proof *.
+
 declare module Adv <: ADV{-OrReal, -OrIdeal, -Reduct}.
 
-local module Hybrid : HYBRID = {
+local module DDHOr1 : GHP.OR = {  (* real *)
+  proc init() : unit = { }
+
+  proc f() : key * key * key = {
+    var x, y : exp;
+    x <$ dexp; y <$ dexp;
+    return (g ^ x, g ^ y, g ^ (x * y));
+  }
+}.
+
+local module DDHOr2 : GHP.OR = {  (* ideal *)
+  proc init() : unit = { }
+
+  proc f() : key * key * key = {
+    var x, y, z : exp;
+    x <$ dexp; y <$ dexp; z <$ dexp;
+    return (g ^ x, g ^ y, g ^ z);
+  }
+}.
+
+local module (Hybrid : GHP.HYBRID_PARAM) (GHOr : GHP.OR) = {
   var i : int
 
   module Or = {
@@ -257,68 +310,94 @@ local module Hybrid : HYBRID = {
     proc get() : key * key * key = {
       var r : key * key * key;
       var x, y, z : exp;
-      if (ctr < m) {
-        if (ctr + 1 < i) {
+      if (ctr <= m) {
+        if (ctr < i) {
           x <$ dexp; y <$ dexp; z <$ dexp;  (* ideal *)
           r <- (g ^ x, g ^ y, g ^ z);
         }
+        elif (ctr = i) { r <@ GHOr.f(); }
         else {
           x <$ dexp; y <$ dexp;  (* real *)
           r <- (g ^ x, g ^ y, g ^ (x * y));
         }
         ctr <- ctr + 1;
       }
-      else {
-        r <- witness;
-      }
+      else { r <- witness; }
       return r;
     }
   }
 
   (* i' should be between 1 and m + 1 *)
 
-  proc main(i' : int) : bool = {
+  proc main(x : unit, i' : int) : bool = {
     var b : bool;
-    i <- i'; Or.ctr <- 0;
+    i <- i'; Or.ctr <- 1;
     b <@ Adv(Or).disting();
     return b;
   }
 }.
 
 local lemma GReal_Hybrid &m :
-  Pr[GReal(Adv).main() @ &m : res] = Pr[Hybrid.main(1) @ &m : res].
+  Pr[GReal(Adv).main() @ &m : res] =
+  Pr[GHP.Exper(Hybrid, DDHOr1).main((), 1) @ &m : res].
 proof.
-byequiv => //; proc; inline.
-seq 1 2 :
+byequiv => //; proc; inline; wp.
+seq 1 4 :
   (={glob Adv} /\ OrReal.ctr{1} = Hybrid.Or.ctr{2} /\
-   OrReal.ctr{1} = 0 /\ Hybrid.i{2} = 1); first auto.
+   OrReal.ctr{1} = 1 /\ Hybrid.i{2} = 1); first auto.
 call
-  (_ :
+  (:
    OrReal.ctr{1} = Hybrid.Or.ctr{2} /\
-   0 <= OrReal.ctr{1} <= m /\ Hybrid.i{2} = 1).
-proc; if => //.
+   1 <= OrReal.ctr{1} <= m + 1 /\ Hybrid.i{2} = 1);
+  last auto; smt(ge1_m).
+proc; if => //; last auto; smt(ge1_m).
 rcondf{2} 1; first auto; smt().
-auto; smt().
-auto.
-auto; smt(ge1_m).
+by if{2}; [inline{2} 1; auto; smt() | auto; smt()].
 qed.
 
 local lemma Hybrid_GIdeal &m :
-  Pr[Hybrid.main(m + 1) @ &m : res] = Pr[GIdeal(Adv).main() @ &m : res].
+  Pr[GHP.Exper(Hybrid, DDHOr1).main((), m + 1) @ &m : res] =
+  Pr[GIdeal(Adv).main() @ &m : res].
 proof.
-byequiv => //; proc; inline.
-seq 2 1 :
+byequiv => //; proc; inline; wp.
+seq 4 1 :
   (={glob Adv} /\ Hybrid.Or.ctr{1} = OrIdeal.ctr{2} /\
-   OrIdeal.ctr{2} = 0 /\ Hybrid.i{1} = m + 1); first auto.
+   OrIdeal.ctr{2} = 1 /\ Hybrid.i{1} = m + 1); first auto.
 call
-  (_ :
+  (:
    Hybrid.Or.ctr{1} = OrIdeal.ctr{2} /\
-   0 <= OrIdeal.ctr{2} <= m /\ Hybrid.i{1} = m + 1).
-proc; if => //.
+   0 <= OrIdeal.ctr{2} <= m + 1 /\ Hybrid.i{1} = m + 1);
+  last auto; smt(ge1_m).
+proc; if => //; last auto.
 rcondt{1} 1; first auto; smt().
-auto; smt().
-auto.
-auto; smt(ge1_m).
+by auto; smt().
+qed.
+
+local lemma Hybrid_step (j : int) &m :
+  1 <= j <= m =>
+  Pr[GHP.Exper(Hybrid, DDHOr2).main((), j) @ &m : res] =
+  Pr[GHP.Exper(Hybrid, DDHOr1).main((), j + 1) @ &m : res].
+proof.
+move => j_rng; byequiv => //; proc; inline; wp.
+seq 4 4 :
+  (Hybrid.i{1} = j /\ Hybrid.i{2} = j + 1 /\
+   Hybrid.Or.ctr{1} = 1 /\ ={glob Adv, Hybrid.Or.ctr});
+  first auto.
+call
+  (:
+   ={Hybrid.Or.ctr} /\ Hybrid.i{1} = j /\
+   Hybrid.i{2} = j + 1 /\ 1 <= Hybrid.Or.ctr{1} <= m + 1);
+  last auto; smt().
+proc.
+if => //; last auto.
+if{1}.
++ rcondt{2} 1; first auto; smt().
+  by auto; smt().
+if{1}.
++ rcondt{2} 1; first auto; smt().
+  by inline{1} 1; auto; smt().
+rcondf{2} 1; first auto; smt().
+by if{2}; [inline{2} 1; auto; smt() | auto; smt()].
 qed.
 
 (* in our sequences of games, we need to shift from lazy to eager
@@ -330,19 +409,18 @@ local clone FullRO with
   type in_t    <- ro_in_t,
   type out_t   <- exp,
   op dout      <- fun _ => dexp,
-  type d_in_t  <- unit,
+  type d_in_t  <- int,
   type d_out_t <- bool
 proof *.
 
 (* first, the sequence of games proving:
 
-   1 <= i < m + 1 => Reduct.i{m} = i =>
-   Pr[Hybrid.main(i) @ &m : res] =
-   Pr[DDH1(Reduct(Adv)).main() @ &m : res] *)
+   1 <= i < m + 1 =>
+   Pr[GHP.Exper(Hybrid, DDHOr1).main((), i) @ &m : res] =
+   Pr[DDH1(Reduct(Adv)).main((), i) @ &m : res]. *)
 
 local module (RO_Disting1 : FullRO.RO_Distinguisher) (RO : FullRO.RO) = {
   var i : int
-  var u, v, w : key
 
   module Or = {
     var ctr : int
@@ -352,12 +430,12 @@ local module (RO_Disting1 : FullRO.RO_Distinguisher) (RO : FullRO.RO) = {
     proc get() : key * key * key = {
       var r : key * key * key;
       var x, y, z : exp;
-      if (ctr < m) {
-        if (ctr + 1 < i) {
+      if (ctr <= m) {
+        if (ctr < i) {
           x <$ dexp; y <$ dexp; z <$ dexp;
           r <- (g ^ x, g ^ y, g ^ z);
         }
-        elif (ctr + 1 = i) {
+        elif (ctr = i) {
           x <@ RO.get(A); y <@ RO.get(B);
           r <- (g ^ x, g ^ y, g ^ (x * y));
         }
@@ -367,136 +445,130 @@ local module (RO_Disting1 : FullRO.RO_Distinguisher) (RO : FullRO.RO) = {
         }
         ctr <- ctr + 1;
       }
-      else {
-        r <- witness;
-      }
+      else { r <- witness; }
       return r;
     }
   }
 
-  proc distinguish() : bool = {
+  proc distinguish(i' : int) : bool = {
     var b : bool;
-    Or.ctr <- 0;
-    RO.sample(A); RO.sample(B); RO.sample(C);
+    i <- i'; Or.ctr <- 1;
+    RO.sample(A); RO.sample(B);
     b <@ Adv(Or).disting();
     return b;
   }
 }.
 
-local lemma Hybrid_MainD_RO_Disting1_RO (i : int) :
-  1 <= i < m + 1 =>
+local lemma Hybrid_DDHOr1_MainD_RO_Disting1_RO (i' : int) :
+  1 <= i' < m + 1 =>
   equiv
-  [Hybrid.main ~
+  [GHP.Exper(Hybrid, DDHOr1).main ~
    FullRO.MainD(RO_Disting1, FullRO.RO).distinguish :
-   ={glob Adv} /\ i'{1} = i /\ RO_Disting1.i{2} = i ==>
+   ={glob Adv} /\ i{1} = i' /\ x{2} = i' ==>
    ={res}].
 proof.
-move => [ge1_i le_i_m]; rewrite ltzS in le_i_m.
+move => [ge1_i' le_i'_m]; rewrite ltzS in le_i'_m.
 transitivity
-  FullRO.MainD(RO_Disting1, FullRO.LRO).distinguish 
-  (={glob Adv} /\ i'{1} = i /\ RO_Disting1.i{2} = i ==> ={res})
-  (={glob Adv} /\ ={glob RO_Disting1} ==> ={res}) => //.
-progress.
-by exists (glob Adv){2} arg{1} RO_Disting1.u{2} RO_Disting1.v{2}
-          RO_Disting1.w{2} RO_Disting1.Or.ctr{2}.
-proc; inline*; wp.
-seq 2 6 :
-  (={glob Adv} /\ Hybrid.i{1} = i /\ RO_Disting1.i{2} = i /\
-   Hybrid.Or.ctr{1} = 0 /\ RO_Disting1.Or.ctr{2} = 0 /\
-   FullRO.RO.m{2} = empty); first auto.
-call
-  (_ :
-   Hybrid.Or.ctr{1} = RO_Disting1.Or.ctr{2} /\
-   0 <= Hybrid.Or.ctr{1} <= m /\
-   Hybrid.i{1} = i /\ RO_Disting1.i{2} = i /\
-   (Hybrid.Or.ctr{1} + 1 <= i => FullRO.RO.m{2} = empty)).
-proc; if => //.
-case (Hybrid.Or.ctr{1} + 1 = Hybrid.i{1}).
-rcondf{1} 1; first auto.
-rcondf{2} 1; first auto; smt().
-rcondt{2} 1; first auto.
-wp; inline*.
-swap{2} 2 -1; swap{2} 6 -4. 
-seq 2 3 :
-  (#pre /\ x{1} = r0{2} /\ y{1} = r1{2} /\
-   x0{2} = A); first auto.
-rcondt{2} 1; first auto; smt(mem_empty).
-sp 0 3.
-rcondt{2} 1; first auto; smt(mem_set mem_empty).
-auto; smt(get_set_sameE).
-if => //; first auto; smt().
-rcondf{2} 1; first auto.
-auto; smt().
-auto.
-auto.
-smt(ge1_m).
+  FullRO.MainD(RO_Disting1, FullRO.LRO).distinguish
+  (={glob Adv} /\ i{1} = i' /\ x{2} = i' ==> ={res})
+  (={glob RO_Disting1, x} ==> ={res}) => //; first smt().
++ proc; inline*; wp.
+  seq 4 6 :
+    (={glob Adv} /\ Hybrid.i{1} = i' /\ RO_Disting1.i{2} = i' /\
+     Hybrid.Or.ctr{1} = 1 /\ RO_Disting1.Or.ctr{2} = 1 /\
+     FullRO.RO.m{2} = empty); first auto.
+  call
+    (:
+     Hybrid.Or.ctr{1} = RO_Disting1.Or.ctr{2} /\
+     1 <= Hybrid.Or.ctr{1} <= m + 1 /\
+     Hybrid.i{1} = i' /\ RO_Disting1.i{2} = i' /\
+     (Hybrid.Or.ctr{1} <= i' => FullRO.RO.m{2} = empty));
+    last auto; smt().
+  proc.
+  if => //; last auto.
+  if => //; first auto; smt().
+  if => //; last auto; smt().
+  inline*; swap{2} 2 -1; swap{2} 6 -4.
+  seq 2 3 :
+    (#pre /\ x0{1} = r0{2} /\ y0{1} = r1{2} /\
+     x0{2} = A); first auto.
+  rcondt{2} 1; first auto; smt(mem_empty).
+  sp 0 3.
+  rcondt{2} 1; first auto; smt(mem_set mem_empty).
+  by auto; smt(get_set_sameE).
 symmetry.
 conseq (FullRO.FullEager.RO_LRO RO_Disting1 _) => //.
-move => _; apply dexp_ll.
+by move => _; apply dexp_ll.
 qed.
 
-local lemma MainD_RO_Disting1_RO_DDH1_Reduct :
+local lemma MainD_RO_Disting1_RO_DDH1_Reduct (i' : int) :
+  1 <= i' < m + 1 =>
   equiv
   [FullRO.MainD(RO_Disting1, FullRO.RO).distinguish ~
    DDH1(Reduct(Adv)).main :
-   ={glob Adv} /\ RO_Disting1.i{1} = Reduct.i{2} ==>
+   ={glob Adv} /\ x{1} = i' /\ i{2} = i' ==>
    ={res}].
 proof.
-proc; inline*; wp.
-swap{1} 6 -5; swap{1} 10 -8; swap{1} 14 -11.
-seq 15 9 :
-  (={glob Adv} /\ RO_Disting1.i{1} = Reduct.i{2} /\
+move => [ge1_i' le_i'_m]; rewrite ltzS in le_i'_m.
+proc; inline*; wp; swap{1} 7 -6; swap{1} 11 -9.
+seq 2 2 : (#pre /\ r0{1} = q1{2} /\ r1{1} = q2{2});
+  first auto.
+seq 10 9 :
+  (={glob Adv} /\
+   RO_Disting1.i{1} = i' /\ Reduct.i{2} = i' /\
    RO_Disting1.Or.ctr{1} = Reduct.Or.ctr{2} /\
    FullRO.RO.m{1}.[A] = Some q1{2} /\
    FullRO.RO.m{1}.[B] = Some q2{2} /\
    Reduct.u{2} = g ^ q1{2} /\
    Reduct.v{2} = g ^ q2{2} /\
    Reduct.w{2} = g ^ (q1{2} * q2{2})).
-wp => /=; rnd{1}; rnd; rnd.
-auto; smt(get_setE mem_set mem_empty).
++ by auto; smt(get_setE mem_set mem_empty).
 exlim q1{2}, q2{2} => q1_R q2_R.
 call
-  (_ :
-   RO_Disting1.i{1} = Reduct.i{2} /\
+  (:
+   RO_Disting1.i{1} = i' /\
+   Reduct.i{2} = i' /\
    RO_Disting1.Or.ctr{1} = Reduct.Or.ctr{2} /\
    FullRO.RO.m{1}.[A] = Some q1_R /\
    FullRO.RO.m{1}.[B] = Some q2_R /\
    Reduct.u{2} = g ^ q1_R /\
    Reduct.v{2} = g ^ q2_R /\
-   Reduct.w{2} = g ^ (q1_R * q2_R)).
-proc; if => //.
-if => //; first auto.
-if => //.
-wp; inline*; auto; smt(get_setE).
-auto.
-auto.
-auto.
+   Reduct.w{2} = g ^ (q1_R * q2_R)); last auto.
+proc.
+if => //; last auto.
+if => //; first auto; smt().
+if => //; last auto.
+inline*.
+rcondf{1} 3; first auto; smt().
+rcondf{1} 6; first auto; smt().
+by auto; smt().
 qed.
 
-local lemma Hybrid_DDH1_Reduct (i : int) &m :
-  1 <= i < m + 1 => Reduct.i{m} = i =>
-  Pr[Hybrid.main(i) @ &m : res] =
-  Pr[DDH1(Reduct(Adv)).main() @ &m : res].
+local lemma reduct1 (i' : int) &m :
+  1 <= i' < m + 1 =>
+  Pr[GHP.Exper(Hybrid, DDHOr1).main((), i') @ &m : res] =
+  Pr[DDH1(Reduct(Adv)).main(i') @ &m : res].
 proof.
-move => i_bnd Reduct_i_eq_i.
-byequiv (_ : ={glob Adv} /\ i'{1} = i /\ Reduct.i{2} = i ==> _) => //.
+move => i'_rng.
+byequiv
+  (: ={glob Adv} /\ i{1} = i' /\ i{2} = i' ==> _) => //.
 transitivity
   FullRO.MainD(RO_Disting1, FullRO.RO).distinguish
-  (={glob Adv} /\ i'{1} = i /\ RO_Disting1.i{2} = i ==> ={res})
-  (={glob Adv} /\ RO_Disting1.i{1} = Reduct.i{2} ==> ={res}) => //.
-progress; by exists (glob Adv){2} arg{1}.
-by apply Hybrid_MainD_RO_Disting1_RO.
+  (={glob Adv} /\ i{1} = i' /\ x{2} = i' ==> ={res})
+  (={glob Adv} /\ x{1} = i' /\ i{2} = i' ==> ={res}) => //.
+by smt().
+by apply Hybrid_DDHOr1_MainD_RO_Disting1_RO.
 by apply MainD_RO_Disting1_RO_DDH1_Reduct.
 qed.
 
-(* next the sequence of games proving:
-   1 <= i < m + 1 => Reduct.i{m} = i =>
-   Pr[Hybrid.main(i + 1) @ &m : res] =
-   Pr[DDH2(Reduct(Adv)).main() @ &m : res] *)
+(* second, the sequence of games proving:
+
+   1 <= i < m + 1 =>
+   Pr[GHP.Exper(Hybrid, DDHOr2).main((), i) @ &m : res] =
+   Pr[DDH2(Reduct(Adv)).main((), i) @ &m : res]. *)
 
 local module (RO_Disting2 : FullRO.RO_Distinguisher) (RO : FullRO.RO) = {
   var i : int
-  var u, v, w : key
 
   module Or = {
     var ctr : int
@@ -506,12 +578,12 @@ local module (RO_Disting2 : FullRO.RO_Distinguisher) (RO : FullRO.RO) = {
     proc get() : key * key * key = {
       var r : key * key * key;
       var x, y, z : exp;
-      if (ctr < m) {
-        if (ctr + 1 < i) {
+      if (ctr <= m) {
+        if (ctr < i) {
           x <$ dexp; y <$ dexp; z <$ dexp;
           r <- (g ^ x, g ^ y, g ^ z);
         }
-        elif (ctr + 1 = i) {
+        elif (ctr = i) {
           x <@ RO.get(A); y <@ RO.get(B); z <@ RO.get(C);
           r <- (g ^ x, g ^ y, g ^ z);
         }
@@ -521,84 +593,80 @@ local module (RO_Disting2 : FullRO.RO_Distinguisher) (RO : FullRO.RO) = {
         }
         ctr <- ctr + 1;
       }
-      else {
-        r <- witness;
-      }
+      else { r <- witness; }
       return r;
     }
   }
 
-  proc distinguish() : bool = {
+  proc distinguish(i' : int) : bool = {
     var b : bool;
-    Or.ctr <- 0;
+    i <- i'; Or.ctr <- 1;
     RO.sample(A); RO.sample(B); RO.sample(C);
     b <@ Adv(Or).disting();
     return b;
   }
 }.
 
-local lemma Hybrid_MainD_RO_Disting2_RO (i : int) :
-  1 <= i < m + 1 =>
+local lemma Hybrid_DDHOr2_MainD_RO_Disting2_RO (i' : int) :
+  1 <= i' < m + 1 =>
   equiv
-  [Hybrid.main ~
+  [GHP.Exper(Hybrid, DDHOr2).main ~
    FullRO.MainD(RO_Disting2, FullRO.RO).distinguish :
-   ={glob Adv} /\ i'{1} = i + 1 /\ RO_Disting2.i{2} = i ==>
+   ={glob Adv} /\ i{1} = i' /\ x{2} = i' ==>
    ={res}].
 proof.
-move => [ge1_i le_i_m]; rewrite ltzS in le_i_m.
+move => [ge1_i' le_i'_m]; rewrite ltzS in le_i'_m.
 transitivity
-  FullRO.MainD(RO_Disting2, FullRO.LRO).distinguish 
-  (={glob Adv} /\ i'{1} = i + 1 /\ RO_Disting2.i{2} = i ==> ={res})
-  (={glob Adv} /\ ={glob RO_Disting2} ==> ={res}) => //.
-progress.
-by exists (glob Adv){2} RO_Disting2.i{2} RO_Disting2.u{2} RO_Disting2.v{2}
-          RO_Disting2.w{2} RO_Disting2.Or.ctr{2}.
-proc; inline*; wp.
-seq 2 6 :
-  (={glob Adv} /\ Hybrid.i{1} = i + 1 /\ RO_Disting2.i{2} = i /\
-   Hybrid.Or.ctr{1} = 0 /\ RO_Disting2.Or.ctr{2} = 0 /\
-   FullRO.RO.m{2} = empty); first auto.
-call
-  (_ :
-   Hybrid.Or.ctr{1} = RO_Disting2.Or.ctr{2} /\
-   0 <= Hybrid.Or.ctr{1} <= m /\
-   Hybrid.i{1} = i + 1 /\ RO_Disting2.i{2} = i /\
-   (Hybrid.Or.ctr{1} + 1 <= i => FullRO.RO.m{2} = empty)).
-proc; if => //.
-if{1}.
-if{2}; first auto; smt().
-rcondt{2} 1; first auto; smt().
-wp; inline*; swap{2} 2 -1; swap{2} 6 -4; swap{2} 10 -7.
-seq 3 4 :
-  (#pre /\ x{1} = r0{2} /\ y{1} = r1{2} /\ z{1} = r2{2} /\
-   x0{2} = A); first auto.
-rcondt{2} 1; first auto; smt(mem_empty).
-sp 0 3.
-rcondt{2} 1; first auto; smt(mem_set mem_empty).
-sp 0 3.
-rcondt{2} 1; first auto; smt(mem_set mem_empty).
-auto; smt(get_set_sameE).
-rcondf{2} 1; first auto; smt().
-rcondf{2} 1; first auto; smt().
-auto; smt().
-auto.
-auto; smt(ge1_m).
+  FullRO.MainD(RO_Disting2, FullRO.LRO).distinguish
+  (={glob Adv} /\ i{1} = i' /\ x{2} = i' ==> ={res})
+  (={glob RO_Disting2, x} ==> ={res}) => //; first smt().
++ proc; inline*; wp.
+  seq 4 7 :
+    (={glob Adv} /\ Hybrid.i{1} = i' /\ RO_Disting2.i{2} = i' /\
+     Hybrid.Or.ctr{1} = 1 /\ RO_Disting2.Or.ctr{2} = 1 /\
+     FullRO.RO.m{2} = empty); first auto.
+  call
+    (:
+     Hybrid.Or.ctr{1} = RO_Disting2.Or.ctr{2} /\
+     1 <= Hybrid.Or.ctr{1} <= m + 1 /\
+     Hybrid.i{1} = i' /\ RO_Disting2.i{2} = i' /\
+     (Hybrid.Or.ctr{1} <= i' => FullRO.RO.m{2} = empty));
+    last auto; smt().
+  proc.
+  if => //; last auto.
+  if => //; first auto; smt().
+  if => //; last auto; smt().
+  inline*; swap{2} 2 -1; swap{2} 6 -4; swap{2} 10 -7.
+  seq 3 4 :
+    (#pre /\ x0{1} = r0{2} /\ y0{1} = r1{2} /\
+     z0{1} = r2{2} /\ x0{2} = A); first auto.
+  rcondt{2} 1; first auto; smt(mem_empty).
+  sp 0 3.
+  rcondt{2} 1; first auto; smt(mem_set mem_empty).
+  sp 0 3.
+  rcondt{2} 1; first auto; smt(mem_set mem_empty).
+  auto; smt(get_set_sameE).
 symmetry.
 conseq (FullRO.FullEager.RO_LRO RO_Disting2 _) => //.
-move => _; apply dexp_ll.
+by move => _; apply dexp_ll.
 qed.
 
-local lemma MainD_RO_Disting2_RO_DDH2_Reduct :
+local lemma MainD_RO_Disting2_RO_DDH2_Reduct (i' : int) :
+  1 <= i' < m + 1 =>
   equiv
   [FullRO.MainD(RO_Disting2, FullRO.RO).distinguish ~
    DDH2(Reduct(Adv)).main :
-   ={glob Adv} /\ RO_Disting2.i{1} = Reduct.i{2} ==>
+   ={glob Adv} /\ x{1} = i' /\ i{2} = i' ==>
    ={res}].
 proof.
-proc; inline*; wp.
-swap{1} 6 -5; swap{1} 10 -8; swap{1} 14 -11.
-seq 15 10 :
-  (={glob Adv} /\ RO_Disting2.i{1} = Reduct.i{2} /\
+move => [ge1_i' le_i'_m]; rewrite ltzS in le_i'_m.
+proc; inline*; wp; swap{1} 7 -6; swap{1} 11 -9; swap{1} 15 -12.
+seq 3 3 :
+  (#pre /\ r0{1} = q1{2} /\ r1{1} = q2{2} /\
+   r2{1} = q3{2}); first auto.
+seq 13 9 :
+  (={glob Adv} /\
+   RO_Disting2.i{1} = i' /\ Reduct.i{2} = i' /\
    RO_Disting2.Or.ctr{1} = Reduct.Or.ctr{2} /\
    FullRO.RO.m{1}.[A] = Some q1{2} /\
    FullRO.RO.m{1}.[B] = Some q2{2} /\
@@ -606,100 +674,93 @@ seq 15 10 :
    Reduct.u{2} = g ^ q1{2} /\
    Reduct.v{2} = g ^ q2{2} /\
    Reduct.w{2} = g ^ q3{2}).
-wp => /=; rnd; rnd; rnd.
-auto; smt(get_setE mem_set mem_empty).
++ auto; smt(get_setE mem_set mem_empty).
 exlim q1{2}, q2{2}, q3{2} => q1_R q2_R q3_R.
 call
-  (_ :
-   RO_Disting2.i{1} = Reduct.i{2} /\
+  (:
+   RO_Disting2.i{1} = i' /\
+   Reduct.i{2} = i' /\
    RO_Disting2.Or.ctr{1} = Reduct.Or.ctr{2} /\
    FullRO.RO.m{1}.[A] = Some q1_R /\
    FullRO.RO.m{1}.[B] = Some q2_R /\
    FullRO.RO.m{1}.[C] = Some q3_R /\
    Reduct.u{2} = g ^ q1_R /\
    Reduct.v{2} = g ^ q2_R /\
-   Reduct.w{2} = g ^ q3_R).
-proc; if => //.
-if => //; first auto.
-if => //; first wp; inline*; auto; smt(get_setE).
-auto.
-auto.
-auto.
+   Reduct.w{2} = g ^ q3_R); last auto.
+proc.
+if => //; last auto.
+if => //; first auto; smt().
+if => //; last auto.
+inline*.
+rcondf{1} 3; first auto; smt().
+rcondf{1} 6; first auto; smt().
+rcondf{1} 9; first auto; smt().
+by auto; smt().
 qed.
 
-local lemma Hybrid_DDH2_Reduct (i : int) &m :
-  1 <= i < m + 1 => Reduct.i{m} = i =>
-  Pr[Hybrid.main(i + 1) @ &m : res] =
-  Pr[DDH2(Reduct(Adv)).main() @ &m : res].
+local lemma reduct2 (i' : int) &m :
+  1 <= i' < m + 1 =>
+  Pr[GHP.Exper(Hybrid, DDHOr2).main((), i') @ &m : res] =
+  Pr[DDH2(Reduct(Adv)).main(i') @ &m : res].
 proof.
-move => i_bnd H.
-byequiv (_ : ={glob Adv} /\ i'{1} = i + 1 /\ Reduct.i{2} = i ==> _) => //.
+move => i'_rng.
+byequiv
+  (: ={glob Adv} /\ i{1} = i' /\ i{2} = i' ==> _) => //.
 transitivity
   FullRO.MainD(RO_Disting2, FullRO.RO).distinguish
-  (={glob Adv} /\ i'{1} = i + 1 /\ RO_Disting2.i{2} = i ==> ={res})
-  (={glob Adv} /\ RO_Disting2.i{1} = Reduct.i{2} ==> ={res}) => //.
-progress; by exists (glob Adv){2} Reduct.i{2}.
-by apply (Hybrid_MainD_RO_Disting2_RO i).
+  (={glob Adv} /\ i{1} = i' /\ x{2} = i' ==> ={res})
+  (={glob Adv} /\ x{1} = i' /\ i{2} = i' ==> ={res}) => //.
+by smt().
+by apply Hybrid_DDHOr2_MainD_RO_Disting2_RO.
 by apply MainD_RO_Disting2_RO_DDH2_Reduct.
-qed.
-
-local lemma Hybrid_DDH1Reduct (i' : int) &m :
-  1 <= i' < m + 1 =>
-  Pr[Hybrid.main(i') @ &m : res] =
-  Pr[DDH1Reduct(Adv).main(i') @ &m : res].
-proof.
-move => ge1_i'_lt_m_plus1.
-rewrite eq_sym.
-byphoare (_ : i = i' /\ glob Adv = (glob Adv){m} ==> _) => //.
-proc; sp.
-call (_ : Reduct.i = i' /\ (glob Adv) = (glob Adv){m} ==> res).
-bypr => &n [] Reduct_i_n_eq_i' eq_glob_n_m.
-rewrite -(Hybrid_DDH1_Reduct i' &n) => //.
-byequiv => //; sim.
-auto.
-qed.
-
-local lemma Hybrid_DDH2Reduct (i' : int) &m :
-  1 <= i' < m + 1 =>
-  Pr[Hybrid.main(i' + 1) @ &m : res] =
-  Pr[DDH2Reduct(Adv).main(i') @ &m : res].
-proof.
-move => ge1_i'_lt_m_plus1.
-rewrite eq_sym.
-byphoare (_ : i = i' /\ glob Adv = (glob Adv){m} ==> _) => //.
-proc; sp.
-call (_ : Reduct.i = i' /\ (glob Adv) = (glob Adv){m} ==> res).
-bypr => &n [] Reduct_i_n_eq_i' eq_glob_n_m.
-rewrite -(Hybrid_DDH2_Reduct i' &n) => //.
-byequiv => //; sim.
-auto.
 qed.
 
 lemma GReal_GIdeal_sect &m :
   `|Pr[GReal(Adv).main() @ &m : res] -
-    Pr[GIdeal(Adv).main() @ &m : res]| <=
-  bigi predT
-  (fun i =>
-   `|Pr[DDH1Reduct(Adv).main(i) @ &m : res] -
-     Pr[DDH2Reduct(Adv).main(i) @ &m : res]|)
-  1 (m + 1).
+    Pr[GIdeal(Adv).main() @ &m : res]| =
+  m%r *
+  `|bigi predT
+    (fun (i : int) =>
+       Pr[DDH1(Reduct(Adv)).main(i) @ &m : res] / m%r)
+    1 (m + 1) -
+    bigi predT
+    (fun (i : int) =>
+       Pr[DDH2(Reduct(Adv)).main(i) @ &m : res] / m%r)
+    1 (m + 1)|.
 proof.
-rewrite GReal_Hybrid -Hybrid_GIdeal (hybrid_gen _ _ Hybrid _ _ _).
-smt(ge1_m).
-move => i bnd_i /=.
-by rewrite Hybrid_DDH1Reduct // Hybrid_DDH2Reduct.
+rewrite GReal_Hybrid -Hybrid_GIdeal.
+rewrite (GHP.hybrid_param () (m + 1) DDHOr1 DDHOr2 Hybrid) /=.
++ by smt(ge1_m).
++ move => i i_rng; rewrite Hybrid_step /#.
+rewrite
+  (eq_big_int _ _
+   (fun (j : int) =>
+      Pr[GHP.Exper(Hybrid, DDHOr1).main(tt, j) @ &m : res] / m%r)
+   (fun (i : int) =>
+      Pr[DDH1(Reduct(Adv)).main(i) @ &m : res] / m%r)).
++ by move => i i_rng /=; rewrite reduct1.
+rewrite
+  (eq_big_int _ _
+   (fun (j : int) =>
+      Pr[GHP.Exper(Hybrid, DDHOr2).main(tt, j) @ &m : res] / m%r)
+   (fun (i : int) =>
+      Pr[DDH2(Reduct(Adv)).main(i) @ &m : res] / m%r)).
++ by move => i i_rng /=; rewrite reduct2.
+done.
 qed.
 
 end section.
 
 lemma GReal_GIdeal (Adv <: ADV{-OrReal, -OrIdeal, -Reduct}) &m :
   `|Pr[GReal(Adv).main() @ &m : res] -
-    Pr[GIdeal(Adv).main() @ &m : res]| <=
-  bigi predT
-  (fun i =>
-   `|Pr[DDH1Reduct(Adv).main(i) @ &m : res] -
-     Pr[DDH2Reduct(Adv).main(i) @ &m : res]|)
-  1 (m + 1).
-proof.
-apply (GReal_GIdeal_sect Adv).
-qed.
+    Pr[GIdeal(Adv).main() @ &m : res]| =
+  m%r *
+  `|bigi predT
+    (fun (i : int) =>
+       Pr[DDH1(Reduct(Adv)).main(i) @ &m : res] / m%r)
+    1 (m + 1) -
+    bigi predT
+    (fun (i : int) =>
+       Pr[DDH2(Reduct(Adv)).main(i) @ &m : res] / m%r)
+    1 (m + 1)|.
+proof. by apply (GReal_GIdeal_sect Adv). qed.
