theories/crypto/GlobalHybrid.ec
@@ -1,68 +1,163 @@
 (* GlobalHybrid.ec *)
 
-(*^ Consider a module `M` with a `bool`-returning procedure `main`
-    taking an integer `i` as its argument. We consider the result of
-    calling `M` with argument `i`, where `i` is in the range `1 .. n`
-    inclusive, for `n >= 1`, to be the `i`th __global hybrid__,
-    global because its entire behavior, and not just that of an oracle
-    it may use, can be a function of `i`.
+(*^ This theory proves several lemmas about __global__ hybrids,
+    hybrids whose entire behavior, not just that of any oracles they
+    may use, can be a function of the hybrid index `i`.
 
-    This theory provides lemmas for upper bounding the absolute value
-    of the difference of the probabilities of the first and last
-    hybrids returning true, given upper bounds on the absolute values
-    of the probability differences for each of the steps, as a function
-    of `i`.
-^*)
+    We have a lemma based on the triangular inequality, where the
+    overall upper bound is the sum of the bounds of the individual
+    steps, as well as the specialization of this to the case where
+    each step's bound is the same.
 
-require import AllCore Real StdOrder StdBigop.
+    And we have a lemma for hybrids parameterized by an oracle
+    that gives an equality, not just an upper bound, assuming
+    a natural precondition holds. This lemma is adapted
+    from the Nominal-SSProve paper "Mechanizing Nested Hybrid Arguments",
+    https://eprint.iacr.org/2025/1122 ^*)
+
+require import AllCore Real StdOrder StdBigop Distr.
 import RealOrder Bigreal BRA.
+
+(*& Type of additional input. &*)
+
+type input.
 
 (*& Module type of global hybrids. &*)
 
 module type HYBRID = {
-  (* i is the index of the hybrid, starting from 1 *)
-  proc main(i : int) : bool
+  (* i is the index of the hybrid, starting from 1
+     x is an additional input *)
+  proc main(x : input, i : int) : bool
 }.
 
 (*& General global hybrid lemma; the bound for each step is a function
     of the index. &*)
 
-lemma hybrid_gen (n : int) (p : int -> real) (M <: HYBRID) &m :
+lemma hybrid_gen (x : input) (n : int) (p : int -> real) (M <: HYBRID) &m :
   1 <= n =>
   (forall (i : int),
-   1 <= i < n => 
-   `|Pr[M.main(i) @ &m : res] - Pr[M.main(i + 1) @ &m : res]| <= p i) =>
-  `|Pr[M.main(1) @ &m : res] - Pr[M.main(n) @ &m : res]| <=
+   1 <= i < n =>
+   `|Pr[M.main(x, i) @ &m : res] - Pr[M.main(x, i + 1) @ &m : res]| <= p i) =>
+  `|Pr[M.main(x, 1) @ &m : res] - Pr[M.main(x, n) @ &m : res]| <=
   bigi predT p 1 n.
 proof.
 move => ge1_n step.
 have ind :
   forall (i : int),
   0 <= i => 1 <= i <= n =>
-  `|Pr[M.main(1) @ &m : res] - Pr[M.main(i) @ &m : res]| <= bigi predT p 1 i.
-  elim => [// | i ge0_i IH [_ i_plus1_le_n]].
+  `|Pr[M.main(x, 1) @ &m : res] -
+    Pr[M.main(x, i) @ &m : res]| <= bigi predT p 1 i.
++ elim => [// | i ge0_i IH [_ i_plus1_le_n]].
   case (i = 0) => [-> /= |].
-  by rewrite ger0_norm // big_geq.
+  + by rewrite ger0_norm // big_geq.
   rewrite -lt0n // ltzE /= => ge1_i.
   rewrite big_int_recr //.
   rewrite (ler_trans
-           (`|Pr[M.main(1) @ &m : res] - Pr[M.main(i) @ &m : res]| +
-            `|Pr[M.main(i) @ &m : res] - Pr[M.main(i + 1) @ &m : res]|)).
-  rewrite RealOrder.ler_dist_add.
-  rewrite ler_add 1:IH 1:/# step /#.
+           (`|Pr[M.main(x, 1) @ &m : res] -
+              Pr[M.main(x, i) @ &m : res]| +
+            `|Pr[M.main(x, i) @ &m : res] -
+              Pr[M.main(x, i + 1) @ &m : res]|)).
+  + by rewrite RealOrder.ler_dist_add.
+  by rewrite ler_add 1:IH 1:/# step /#.
 by rewrite ind // (IntOrder.ler_trans 1).
 qed.
 
 (*& Simple global hybrid lemma; the bound for each step is a constant. &*)
 
-lemma hybrid_simp (n : int) (p : real) (M <: HYBRID) &m :
+lemma hybrid_simp (x : input) (n : int) (p : real) (M <: HYBRID) &m :
   1 <= n =>
   (forall (i : int),
-   1 <= i < n => 
-   `|Pr[M.main(i) @ &m : res] - Pr[M.main(i + 1) @ &m : res]| <= p) =>
-  `|Pr[M.main(1) @ &m : res] - Pr[M.main(n) @ &m : res]| <= (n - 1)%r * p.
+   1 <= i < n =>
+   `|Pr[M.main(x, i) @ &m : res] -
+     Pr[M.main(x, i + 1) @ &m : res]| <= p) =>
+  `|Pr[M.main(x, 1) @ &m : res] -
+    Pr[M.main(x, n) @ &m : res]| <= (n - 1)%r * p.
 proof.
 move => ge1_n step.
-have HG := hybrid_gen n (fun _ => p) M &m _ _ => //.
+have HG := hybrid_gen x n (fun _ => p) M &m _ _ => //.
 by rewrite Bigreal.sumri_const in HG.
 qed.
+
+(*& Hybrids parameterized by an oracle. &*)
+
+theory Param.
+
+(*& Types of oracle inputs. &*)
+
+type or_input.
+
+(*& Types of oracle outputs. &*)
+
+type or_output.
+
+(*& Oracle module type. &*)
+
+module type OR = {
+  proc init() : unit
+  proc f(x : or_input) : or_output
+}.
+
+(*& Parameterized hybrid module type. &*)
+
+module type HYBRID_PARAM (Or : OR) = {
+  (* i is the index of the hybrid, starting from 1
+     x is an additional input *)
+  proc main(x : input, i : int) : bool {Or.f}
+}.
+
+(*& Parameterized hybrid experiment. &*)
+
+module Exper(M : HYBRID_PARAM, Or : OR) = {
+  proc main(x : input, i : int) : bool = {
+    var b : bool;
+    Or.init();
+    b <@ M(Or).main(x, i);
+    return b;
+  }
+}.
+
+(*& Parameterized hybrid lemma. &*)
+
+lemma hybrid_param (x : input) (n : int) (Or1 <: OR) (Or2 <: OR)
+                   (M <: HYBRID_PARAM) &m :
+  1 < n =>
+  (forall (i : int),
+   1 <= i < n =>
+   Pr[Exper(M, Or2).main(x, i) @ &m : res] =
+   Pr[Exper(M, Or1).main(x, i + 1) @ &m : res]) =>
+  `|Pr[Exper(M, Or1).main(x, 1) @ &m : res] -
+    Pr[Exper(M, Or1).main(x, n) @ &m : res]| =  (* also Or1 *)
+  (n - 1)%r *
+  `|bigi predT
+    (fun (j : int) => Pr[Exper(M, Or1).main(x, j) @ &m : res] / (n - 1)%r)
+    1 n -
+    bigi predT
+    (fun (j : int) => Pr[Exper(M, Or2).main(x, j) @ &m : res] / (n - 1)%r)
+    1 n|.
+proof.
+move => gt1_n steps.
+rewrite
+  (telescoping_sum
+   (fun i => Pr[Exper(M, Or1).main(x, i) @ &m : res])) 1:/# /=.
+rewrite
+  (eq_big_int _ _ _
+   (fun (i : int) =>
+      Pr[Exper(M, Or1).main(x, i) @ &m : res] -
+      Pr[Exper(M, Or2).main(x, i) @ &m : res]) _).
++ by move => i i_rng /=; rewrite -steps.
+rewrite big_split -sumrN.
+rewrite -normrZ 1:/# RField.mulrC RField.mulrBl 2!mulr_suml /=.
+have -> :
+  (fun (i : int) =>
+     Pr[Exper(M, Or1).main(x, i) @ &m : res] * (n - 1)%r / (n - 1)%r) =
+  (fun (i : int) => Pr[Exper(M, Or1).main(x, i) @ &m : res]).
++ by apply fun_ext => i; rewrite -RField.mulrA Num.Domain.divrr /#.
+have -> :
+  (fun (i : int) =>
+     Pr[Exper(M, Or2).main(x, i) @ &m : res] * (n - 1)%r / (n - 1)%r) =
+  (fun (i : int) => Pr[Exper(M, Or2).main(x, i) @ &m : res]).
++ by apply fun_ext => i; rewrite -RField.mulrA Num.Domain.divrr /#.
+done.
+qed.
+
+end Param.
